sha/HMAC_spec_pad.v
@@ -9,8 +9,6 @@ Require Import hmac_pure_lemmas.
 Require Import ByteBitRelations.
 Require Import HMAC_common_defs.
 
-Module HMAC_Pad.
-
 Local Open Scope program_scope.
 
 Section HMAC.
@@ -129,19 +127,74 @@ Proof.
       eapply app_inv_head. eassumption.
 Qed.
 
-Lemma hash_block_equiv shah hashblock
-     (HHB: shah= fun rgs bl => intsToBits (hashblock (bitsToInts rgs) (bitsToInts bl))):
+Module Type INST.
+Parameter shah : Blist -> Blist ->  Blist.
+Parameter hashblock : list int -> list int -> list int.
+Parameter HHB : shah =
+      (fun rgs bl : Blist =>
+       intsToBits (hashblock (bitsToInts rgs) (bitsToInts bl))).
+
+Parameter hashblocks: list int -> list int -> list int.
+Parameter d:nat.
+
+Parameter HBS_eq : forall r msg : list int,
+         hashblocks r msg =
+         match msg with
+         | [] => r
+         | _ :: _ => hashblocks (hashblock r (firstn d msg)) (skipn d msg)
+         end.
+End INST.
+
+Require Import HMAC_functional_prog. (*Just for HMAC_FUN*)
+
+
+Module HMAC_Pad (HF:HP.HASH_FUNCTION) (I:INST).
+(*Module HMAC_Pad.Declare Module HF:HP.HASH_FUNCTION.*)
+Module HM:= HP.HMAC_FUN HF.
+
+(*Module PadConcrete (HF:HP.HASH_FUNCTION).*)
+
+(*From hmac_common_lemmas TODO: Isolate*)
+(*Lemma SF_ByteRepr x: isbyteZ x ->
+                     HM.sixtyfour x = 
+                     map Byte.unsigned (HM.sixtyfour (Byte.repr x)).
+Proof. intros. unfold HM.sixtyfour.
+ rewrite map_list_repeat.
+ rewrite Byte.unsigned_repr; trivial. destruct H. 
+ assert (BMU: Byte.max_unsigned = 255). reflexivity. omega.
+Qed.
+*)
+(*From hmac_common_lemmas TODO: Isolate*)
+(*Lemma length_SF {A} (a:A) :length (HM.sixtyfour a) = HF.BlockSize.
+Proof. apply length_list_repeat. Qed. 
+*)
+(*From SHaInstantiation -- TODO: Isolate*)
+Lemma xor_equiv_byte: forall xpad XPAD k K, isbyteZ XPAD ->
+                          bytes_bits_lists xpad (HM.sixtyfour XPAD) ->
+                          length K= HF.BlockSize ->
+                          bytes_bits_lists k (map Byte.unsigned K) ->
+bytes_bits_lists (BLxor k xpad) (HM.mkArgZ K (Byte.repr XPAD)).
+Proof. intros. apply inner_general_mapByte; try assumption.
+       rewrite <- HM.SF_ByteRepr; trivial.
+Qed.
+(*
+Lemma isbyte_hmaccore ipad opad m k: 
+   Forall isbyteZ (HM.HmacCore (Byte.repr ipad) (Byte.repr opad) m k).
+Proof. apply HF.Hash_isbyteZ. Qed. *)
+
+(*Parameter *)
+Lemma hash_block_equiv:
   forall (bits : Blist) (bytes : list Z)
          (regs : Blist) REGS,
     Forall isbyteZ bytes ->
     regs = bytesToBits (intlist_to_Zlist REGS) ->
     bits = bytesToBits bytes ->
-    shah regs bits =
+    I.shah regs bits =
     bytesToBits (intlist_to_Zlist
-                   (hashblock REGS (Zlist_to_intlist bytes))).
+                   (I.hashblock REGS (Zlist_to_intlist bytes))).
 Proof.
   intros bits bytes regs REGS bytes_inrange regs_eq input_eq.
-  subst shah. unfold intsToBits.
+  rewrite I.HHB. unfold intsToBits.
   apply f_equal.
   apply f_equal.
   rewrite -> regs_eq; clear regs_eq.
@@ -155,22 +208,14 @@ Proof.
   * apply isbyte_intlist_to_Zlist. 
 Qed.
 
-(*shah = sha_h, hashblock=hash_block, hashblocks=hash_blocks *)
-Lemma fold_equiv_blocks b (B:(0<b)%nat) d (DB32: (d*32)%nat=b)
-      shah hashblock hashblocks
-     (HHB: shah= fun rgs bl => intsToBits (hashblock (bitsToInts rgs) (bitsToInts bl)))
-     (HBS_eq: forall r msg, hashblocks r msg =
-       match msg with
-       | [] => r
-       | _ :: _ => hashblocks (hashblock r (firstn d msg)) (skipn d msg)
-       end):
+Lemma fold_equiv_blocks b (B:(0<b)%nat) (DB32: (I.d*32)%nat=b):
   forall (l : Blist) (acc : Blist)
          (L : list int) (ACC : list int),
       InBlocks b l ->
-      InBlocks d L ->
+      InBlocks I.d L ->
       l = convert L ->
       acc = convert ACC ->
-      hash_blocks_bits b B shah acc l = convert (hashblocks ACC L).
+      hash_blocks_bits b B I.shah acc l = convert (I.hashblocks ACC L).
 Proof. 
   intros l acc L ACC bit_blocks bytes_blocks inputs_eq acc_eq.
   
@@ -180,13 +225,13 @@ Proof.
     revert acc ACC inputs_eq acc_eq.
     induction bytes_blocks; intros.
 
-    - rewrite HBS_eq.
+    - rewrite I.HBS_eq.
       rewrite -> hash_blocks_bits_equation.
       apply acc_eq. 
     - rewrite -> H0 in *.
       unfold convert in inputs_eq. 
       destruct front.
-      { simpl in H. subst d; omega. }
+      { simpl in H. rewrite <- H in *; omega. }
       { simpl in inputs_eq. inversion inputs_eq. }
 
   *
@@ -202,7 +247,7 @@ Proof.
       { simpl in H. subst b. omega. }
       { simpl in inputs_eq. inversion inputs_eq. }
 
-    - clear IHbytes_blocks. intros. rewrite HBS_eq; clear HBS_eq.
+    - clear IHbytes_blocks. intros. rewrite I.HBS_eq.
       rewrite -> hash_blocks_bits_equation.
       repeat rewrite -> length_not_emp.
       rewrite -> H0.
@@ -215,8 +260,7 @@ Proof.
       + rewrite -> H0 in inputs_eq.
         rewrite -> H2 in inputs_eq.
         eapply (back_equiv DB32); eassumption. 
-      + 
-        rewrite  (@hash_block_equiv _ _ HHB front0 (intlist_to_Zlist front) acc ACC); auto.
+      + rewrite (@hash_block_equiv front0 (intlist_to_Zlist front) acc ACC); auto.
         rewrite -> intlist_to_Zlist_to_intlist.
         reflexivity.
         { apply isbyte_intlist_to_Zlist. }
@@ -227,36 +271,29 @@ Proof.
      + rewrite -> H2. rewrite -> app_length. rewrite -> H1. omega.
 Qed.
 
-Lemma equiv_pad shah shaiv shasplitandpad c p (B: (0< b c p)%nat) d (DB32: (d*32 =b c p)%nat)
-      hashblock hashblocks
-     (HHB: shah= fun rgs bl => intsToBits (hashblock (bitsToInts rgs) (bitsToInts bl)))
-     (HBS_eq: forall r msg, hashblocks r msg =
-       match msg with
-       | [] => r
-       | _ :: _ => hashblocks (hashblock r (firstn d msg)) (skipn d msg)
-       end) 
+Lemma equiv_pad shaiv shasplitandpad c p (B: (0< b c p)%nat) (DB32: (I.d*32 =b c p)%nat)
      ir (IVIR: shaiv = convert ir)
-       gap (GAP: forall bits, NPeano.divide d (length (gap (bitsToBytes bits))))
+       gap (GAP: forall bits, NPeano.divide I.d (length (gap (bitsToBytes bits))))
        (sap_gap: forall bits, shasplitandpad bits = bytesToBits (intlist_to_Zlist (gap (bitsToBytes bits))))
        HASH
-       (HSH: forall (m:list Z), HASH m = intlist_to_Zlist (hashblocks ir (gap m))):
+       (HSH: forall (m:list Z), HASH m = intlist_to_Zlist (I.hashblocks ir (gap m))):
        forall (bits : Blist) (bytes : list Z),
                     bytes_bits_lists bits bytes ->
                     bytes_bits_lists
-                      (hash_words_padded c p B shah shaiv shasplitandpad bits)
+                      (hash_words_padded c p B I.shah shaiv shasplitandpad bits)
                       (HASH bytes).
 Proof.
   intros bits bytes input_eq.
   unfold hash_words_padded.
-  change ((hash_words c p B shah shaiv ∘ shasplitandpad) bits) with
-  (hash_words c p B shah shaiv (shasplitandpad bits)).
+  change ((hash_words c p B I.shah shaiv ∘ shasplitandpad) bits) with
+  (hash_words c p B I.shah shaiv (shasplitandpad bits)).
     unfold hash_words.
     unfold h_star. rewrite HSH; clear HSH. 
     apply bytes_bits_comp_ind.
     { apply isbyte_intlist_to_Zlist. }
     { apply bytes_bits_ind_comp in input_eq.
         { subst bytes. rewrite sap_gap; clear sap_gap.
-          eapply (fold_equiv_blocks B DB32 _ _ HHB HBS_eq).
+          eapply (fold_equiv_blocks B DB32).
           3: reflexivity.
           3: assumption.
           apply InBlocks_len. rewrite bytesToBits_len, length_intlist_to_Zlist.
@@ -269,4 +306,96 @@ Proof.
     }
 Qed.
 
-End HMAC_Pad.
+Theorem HMAC_pad_concrete splitandpad c p (B: (0< b c p)%nat) (BS: (HF.BlockSize * 8)%nat = b c p)
+        (DB32: (I.d*32 =b c p)%nat)
+         ir (*ie initial_regs*) gap (*ie generate_and_pad*)
+         (GAP: forall bits, NPeano.divide I.d (length (gap (bitsToBytes bits))))
+         (sap_gap: forall bits, splitandpad bits = bytesToBits (intlist_to_Zlist (gap (bitsToBytes bits))))
+         (HSH: forall (m:list Z), HF.Hash m = intlist_to_Zlist (I.hashblocks ir (gap m)))
+         (K : list byte) (M H : list Z) (OP IP : Z)
+                          (k m h : Blist) (op ip : Blist) (ipByte: isbyteZ IP) (opByte: isbyteZ OP):
+  length K = HF.BlockSize ->
+  bytes_bits_lists k (map Byte.unsigned K) ->
+  bytes_bits_lists m M ->
+  bytes_bits_lists op (HM.sixtyfour OP) ->
+  bytes_bits_lists ip (HM.sixtyfour IP) ->
+  HMAC c p B I.shah (convert ir) splitandpad op ip k m = h ->
+  HM.HmacCore (Byte.repr IP) (Byte.repr OP) M K = H ->
+  bytes_bits_lists h H.
+Proof.
+  intros padded_key_len padded_keys_eq msgs_eq ops_eq ips_eq HMAC_abstract HMAC_concrete.
+  rewrite <- HMAC_abstract. rewrite <- HMAC_concrete.
+  unfold HMAC. unfold HM.HmacCore. unfold HM.OUTER. unfold HM.INNER.
+  unfold HM.outerArg. unfold HM.innerArg.
+
+  unfold HMAC_2K. unfold GHMAC_2K. rewrite -> split_append_id.
+
+  { eapply equiv_pad.
+    apply DB32. reflexivity. apply GAP. assumption. assumption.
+    apply bytes_bits_lists_append.
+    apply xor_equiv_byte; trivial. 
+
+    eapply equiv_pad. 
+    apply DB32. reflexivity. apply GAP. assumption. assumption.
+    apply bytes_bits_lists_append.
+    - apply xor_equiv_byte; trivial.
+    - assumption. }
+
+  { apply BLxor_length; erewrite bytes_bits_length; try eassumption.
+         rewrite map_length, padded_key_len. apply BS.
+         rewrite HM.length_SF. apply BS. }
+
+  { apply BLxor_length; erewrite bytes_bits_length; try eassumption.
+         rewrite map_length, padded_key_len. apply BS.
+         rewrite HM.length_SF. apply BS. }
+Qed.
+
+Theorem HMAC_pad_concrete' splitandpad c p (B: (0< b c p)%nat) (BS: (HF.BlockSize * 8)%nat =b c p)
+        (DB32: (I.d*32 =b c p)%nat)
+         ir (*ie initial_regs*) gap (*ie generate_and_pad*)
+         (GAP: forall bits, NPeano.divide I.d (length (gap (bitsToBytes bits))))
+         (sap_gap: splitandpad = fun bits => bytesToBits (intlist_to_Zlist (gap (bitsToBytes bits))))
+         (HSH: forall (m:list Z), HF.Hash m = intlist_to_Zlist (I.hashblocks ir (gap m)))
+         (K : list byte) (M : list Z) (OP IP : Z)
+                          (k m : Blist) (op ip : Blist) (ipByte: isbyteZ IP) (opByte: isbyteZ OP):
+  length K = HF.BlockSize ->
+  bytes_bits_lists k (map Byte.unsigned K) ->
+  bytes_bits_lists m M ->
+  bytes_bits_lists op (HM.sixtyfour OP) ->
+  bytes_bits_lists ip (HM.sixtyfour IP) ->
+  bytes_bits_lists
+     (HMAC c p B I.shah (convert ir) splitandpad op ip k m)
+     (HM.HmacCore (Byte.repr IP) (Byte.repr OP) M K).
+Proof.
+  intros. eapply HMAC_pad_concrete; try reflexivity.
+  eassumption. eassumption. eassumption. eassumption. eassumption. eassumption.
+  eassumption. eassumption. eassumption. eassumption. eassumption. rewrite sap_gap. trivial.
+Qed.
+
+End HMAC_Pad. 
+(*
+Lemma equiv_pad_SHA256 HASH c p B sap h iv: forall (bits : Blist) (bytes : list Z),
+                    bytes_bits_lists bits bytes ->
+                    bytes_bits_lists
+                      (HMAC_Pad.hash_words_padded c p B h iv sap bits)
+                      (HASH bytes).
+Proof. intros.
+  eapply HMAC_Pad.equiv_pad (*with (gap:=generate_and_pad')*).
+  2: reflexivity.
+  2: apply hash_blocks_equation.
+  reflexivity. reflexivity.
+  apply gap_divide16.
+  intros. unfold sha_splitandpad. f_equal. 
+    apply bytes_bits_ind_comp in H.
+    { subst bytes. unfold generate_and_pad'.
+      rewrite pure_lemmas.Zlist_to_intlist_to_Zlist; trivial.
+        destruct (pad_len_64_nat (bitsToBytes bits0)). rewrite H.
+          exists ((x*16)%nat). rewrite mult_comm, <- mult_assoc. reflexivity.
+        apply pad_isbyteZ. eapply bitsToBytes_isbyteZ. reflexivity. }
+    apply (bytesBitsLists_isbyteZ _ _ H).
+  intros; unfold HP.SHA256.Hash.
+    rewrite -> functional_prog.SHA_256'_eq. unfold SHA256.SHA_256.
+    rewrite <- pad_compose_equal; reflexivity.
+  assumption.
+Qed.
+*)
